## Building Neural Network from Scratch.

#### 1 : We will create a neural network 

![image info](./pictures/excel 1.png)

In the given image, we are having:

- <b>Inputs</b> : i1, i2 
- <b>First hidden layer before activation</b> : h1,h2
- <b>First hidden layer after activation</b> : a_h1, a_h2
- <b>Output before activation function</b> : o1, o2
- <b>Output after activation</b> : a_o1, o_oh2
- <b>Weights</b> : w1, w2, w3, w4, w5, w6, w7, w8
- <b>Error from first input</b> : E1
- <b>Error from second input</b> : E2
- <b>Error</b> : E_total
- <b>Target</b> : we have two targets, t1 = 0.01 and t2 = 0.99. target is just the output which we are getting here i.e a_o1, a_o2

< Note: Do not have any biased
< Activation layer is not just in hidden layer, it is in all the layers. 

Formulas : 
h1 : w1*i1 + w2 *i2
h2 : w3*i1 :w4*i2
a_h1 : σ(h1)
a_h2 : σ(h2)
o1 : w5*a_h1 + w6*a_h2
o2 : w7*a_h1 + w8*a_h2
a_o1 : σ(o1)
a_o2 : σ(o2)
E1 = ½*(t1-a_o1)²
E2 = ½*(t2-a_o2)²
E_total = E1 + E2

#### Calculate all values and put them in the table.

Calculate all the values inside that table using the above formulas.

< Values Given, 
inputs : i1 = 0.05, i2 = 0.1
outputs : t1 = 0.01, t2 = 0.99
Weights : w1 = 0.15, w2 = 0.2, w3 = 0.25, w4 = 0.3, w5 = 0.4, w6 = 0.45, w7 = 0.5, w8 = 0.55

< Values to be calculated,
We will be calculating these values using the above formulas in our excel sheet.
h1, h2, a_h1, a_h2, o1, o2 , a_o1, a_o2 , E1, E2, E_total, 


Till here, we were calulating forward propagation.Now we will be calculating backward propogation.
To do backward propogation, we will start with <b>∂E_total/∂w5</b>.
In the above equation, we have removed E2 as it is not getting generated by w5. So we will not be using it. w5 is directly linked with E_total, but there are many steps in between. ∂(E1)/∂W5 has two things in between, i.e o1 and a_o1. We will be going through this route.

> ∂E_total/∂w5  = ∂(E1 +E2)/∂W5 
> ∂E_total/∂w5  = ∂(E1)/∂W5

Chain rule, 

< ∂(E1)/∂W5 = ∂(E1)/∂(a_o1) * ∂(a_o1)/∂(o1) * ∂(o1)/∂w5

Now we will calculate the values of the above output.

< 1.

 < ∂(E1)/∂(a_o1) =  ∂(½*(t1-a_o1)²) /  ∂(a_o1)
 < ∂(E1)/∂(a_o1) =  (t1 – a_o1) * (-1)
 < ∂(E1)/∂(a_o1) =   a_o1 - t1

< 2.

 < ∂(a_o1)/∂(o1) =  ∂(σ(o1)) /  ∂(o1)
 < ∂(a_o1)/∂(o1) =  σ(o1) *  (1 -  σ(o1))
 < ∂(a_o1)/∂(o1) =  a_o1 * (1 – a_o1)

< 3.

 < ∂(o1)/∂w5 = ∂(w5 * a_h1 + w6 * a_h2) / ∂w5
 < ∂(o1)/∂w5 = a_h1


Now,
               ∂E_total / ∂w5 = (a_o1 – t1) * a_o1 * (1 – a_o1)) * a_h1

Similarly, we will find the equation for w6, w7, w8.

	   ∂E_total / ∂w6 = (a_o1 – t1) * a_o1 * (1 – a_o1)) * a_h2
               ∂E_total / ∂w7 = (a_o2 – t2) * a_o2 * (1 – a_o2)) * a_h1
               ∂E_total / ∂w8 = (a_o2 – t2) * a_o2 * (1 – a_o2)) * a_h2

Now, we will calculate values for w1, w2, w3, w4.  

Before looking at w1, we will look at a_h1 value because w1 taking  two  routes i.e from a_o1 and a_o2
For that we will first calculate ∂E_total/∂a_h1 then will go to w1.

∂E_total / ∂a_h1 = ∂(E1 + E2) / ∂(a_h1)

This time we are having E1 as well as E2, as we have two routes.

∂(E1) / ∂(a_h1) = ∂E1/∂a_o1 * ∂a_o1/∂o1 * ∂o1/∂a_h1
∂(E1) / ∂(a_h1) = (a_o1 -t1) * (a_o1) * (1-a_o1) *w5

∂(E2) / ∂(a_h1) = ∂E2/∂a_o2 * ∂a_o2/∂o2 * ∂o2/∂a_h1
∂(E2) / ∂(a_h1) = (a_o2 -t2) * (a_o2) * (1-a_o2) *w7

∂E_total / ∂a_h1 = ∂(E1 + E2) / ∂(a_h1)
∂E_total / ∂a_h1 = (a_o1 -t1) * (a_o1) * (1-a_o1) *w5 + (a_o2 -t2) * (a_o2) * (1-a_o2) *w7

Similary, we will calculate for ∂E_total / ∂a_h2

∂E_total / ∂a_h2 = (a_o2 -t2) * (a_o2) * (1-a_o2) *w8 + (a_o1 -t1) * (a_o1) * (1-a_o1) *w6

Now Caluclate ∂E_total/∂w1 

∂E_total/∂w1 = E_total/a_o1 * a_o1/o1 * o1/a_h1 * a_h1/h1 * h1/w1
∂E_total/∂w1 = ∂E_total/∂a_h1 * ∂a_h1/∂h1 * ∂h1/∂w1
∂E_total/∂w1 = ∂E_total/∂a_h1 * a_h1 * (1-a_h1) * ∂h1/∂w1
∂E_total/∂w1 = ∂E_total/∂a_h1 *a_h1 * (1- a_h1)*i1

Similarly calculate for w2, w3 and w4

∂E_total/∂w2 = ∂E_total/∂a_h1 *a_h1 * (1- a_h1)*i2
∂E_total/∂w3 = ∂E_total/∂a_h2 *a_h2 * (1- a_h2)*i1
∂E_total/∂w4 = ∂E_total/∂a_h2 *a_h2 * (1- a_h2)*i2




